WIP

ovn/proofs/ssprove/extraction/Hacspec_ovn.v
@@ -395,6 +395,7 @@ Equations zkp_one_out_of_two {L1 : {fset Location}} {L2 : {fset Location}} {L3 :
 Admit Obligations. (* slow *) (* Solve All Obligations with solve_ssprove_obligations. *)
 Fail Next Obligation.
 
+Obligation Tactic := try timeout 4 solve_ssprove_obligations.
 Equations zkp_one_out_of_two_validate {L1 : {fset Location}} {L2 : {fset Location}} {I1 : Interface} {I2 : Interface} {v_Z : _} {v_G : _} `{ t_Sized (v_Z)} `{ t_Sized (v_G)} `{ t_Z_Field (v_Z)} `{ t_Group (v_G) (v_Z)} (h : both L1 I1 (f_group_type)) (zkp : both L2 I2 (t_OrZKPCommit (v_Z := v_Z) (v_G := v_G))) : both (L1 :|: L2 (* :|: f_eq_loc *) :|: f_div_loc :|: f_g_loc :|: f_g_pow_loc :|: f_hash_loc :|: f_pow_loc :|: f_prod_loc :|: f_add_loc) (I1 :|: I2) ('bool) :=
   zkp_one_out_of_two_validate h zkp  :=
     letb c := f_hash (impl__into_vec (unsize (box_new (array_from_list [f_or_zkp_x zkp;
@@ -460,14 +461,15 @@ Definition cast_vote_state_ret_loc {v_Z : _} {v_G : _} {n : both (fset []) (fset
 Notation Result_Ok_case := inl.
 Notation Result_Err_case := inr.
 (* Obligation Tactic := try timeout 2 solve_ssprove_obligations. *)
-Equations cast_vote {L1 : {fset Location}} {L2 : {fset Location}} {I1 : Interface} {I2 : Interface} {v_Z : _} {v_G : _} {n : both (fset []) (fset []) (uint_size)} {v_A : _} {impl_574521470_ : _} `{ t_Sized (v_Z)} `{ t_Sized (v_G)} `{ t_Sized (v_A)} `{ t_Sized (impl_574521470_)} `{ t_Z_Field (v_Z)} `{ t_Group (v_G) (v_Z)} `{ t_HasActions (v_A)} `{ t_HasReceiveContext (impl_574521470_) ('unit)} (ctx : both L1 I1 (impl_574521470_)) (state : both L2 I2 (t_OvnContractState (v_Z := v_Z) (v_G := v_G) (n := n)(* (both (fset []) (fset []) (uint_size)) *))) : both (L1 :|: L2 :|: fset [cast_vote_state_ret_loc (n := n);prod1_loc (n := n);prod2_loc (n := n)] :|:
-    Hacspec_ovn_Ovn_traits.f_div_loc :|:
-    Hacspec_ovn_Ovn_traits.f_group_one_loc :|:
-    Hacspec_ovn_Ovn_traits.f_prod_loc :|:
-    Hacspec_ovn_Ovn_traits.f_g_pow_loc :|:
-    Hacspec_ovn_Ovn_traits.f_pow_loc :|:
-    Hacspec_ovn_Ovn_traits.f_field_one_loc :|:
-    Hacspec_ovn_Ovn_traits.f_field_zero_loc (* :|: f_get_loc :|: f_clone_loc :|: f_accept_loc :|: f_parameter_cursor_loc *)) (I1 :|: I2) (t_Result ((v_A × t_OvnContractState (v_Z := v_Z) (v_G := v_G) (n := n) (* (both (fset []) (fset []) (uint_size)) *))) (t_ParseError)) :=
+Equations cast_vote {L1 : {fset Location}} {L2 : {fset Location}} {I1 : Interface} {I2 : Interface} {v_Z : _} {v_G : _} {n : both (fset []) (fset []) (uint_size)} {v_A : _} {impl_574521470_ : _} `{ t_Sized (v_Z)} `{ t_Sized (v_G)} `{ t_Sized (v_A)} `{ t_Sized (impl_574521470_)} `{ t_Z_Field (v_Z)} `{ t_Group (v_G) (v_Z)} `{ t_HasActions (v_A)} `{ t_HasReceiveContext (impl_574521470_) ('unit)} (ctx : both L1 I1 (impl_574521470_)) (state : both L2 I2 (t_OvnContractState (v_Z := v_Z) (v_G := v_G) (n := n)(* (both (fset []) (fset []) (uint_size)) *))) : both (L1 :|: L2 :|:
+    f_div_loc :|:
+    f_group_one_loc :|:
+    f_prod_loc :|:
+    f_g_pow_loc :|:
+    f_g_loc :|: f_hash_loc :|: f_mul_loc :|: f_random_field_elem_loc :|: f_sub_loc :|:
+    f_pow_loc :|:
+    f_field_one_loc :|:
+    f_field_zero_loc :|: fset [cast_vote_state_ret_loc (n := n);prod1_loc (n := n);prod2_loc (n := n)] (* :|: f_get_loc :|: f_clone_loc :|: f_accept_loc :|: f_parameter_cursor_loc *)) (I1 :|: I2) (t_Result ((v_A × t_OvnContractState (v_Z := v_Z) (v_G := v_G) (n := n) (* (both (fset []) (fset []) (uint_size)) *))) (t_ParseError)) :=
   cast_vote ctx state  :=
     solve_lift (run (letb '(_,out) := f_get (f_parameter_cursor ctx) in
     letm[choice_typeMonad.result_bind_code (t_Result ((v_A × t_OvnContractState (v_Z := v_Z) (v_G := v_G) (n := n)(* (both (fset []) (fset []) (uint_size)) *))) (t_ParseError))] (params : t_CastVoteParam (v_Z)) := matchb out with
@@ -482,63 +484,120 @@ Equations cast_vote {L1 : {fset Location}} {L2 : {fset Location}} {I1 : Interfac
     ControlFlow_Continue (letb g_pow_yi := compute_g_pow_yi (cast_int (WS2 := U32) (f_cvp_i params)) (f_g_pow_xis state) in
     letb g_pow_xi_yi_vi := compute_group_element_for_vote (f_cvp_xi params) (f_cvp_vote params) g_pow_yi in
     letb zkp_vi := zkp_one_out_of_two (f_cvp_zkp_random_w params) (f_cvp_zkp_random_r params) (f_cvp_zkp_random_d params) g_pow_yi (f_cvp_xi params) (f_cvp_vote params) in
-    letb cast_vote_state_ret loc(cast_vote_state_ret_loc) := f_clone state in
-    letb _ := letb cast_vote_state_ret loc(cast_vote_state_ret_loc) := Build_t_OvnContractState[cast_vote_state_ret] (f_g_pow_xi_yi_vis := update_at_usize (f_g_pow_xi_yi_vis cast_vote_state_ret) (cast_int (WS2 := U32) (f_cvp_i params)) g_pow_xi_yi_vi) in
+    letb cast_vote_state_ret loc(cast_vote_state_ret_loc (n := n)) := f_clone state in
+    letb _ := letb cast_vote_state_ret loc(cast_vote_state_ret_loc (n := n)) := Build_t_OvnContractState[cast_vote_state_ret] (f_g_pow_xi_yi_vis := update_at_usize (f_g_pow_xi_yi_vis cast_vote_state_ret) (cast_int (WS2 := U32) (f_cvp_i params)) g_pow_xi_yi_vi)(*  : both (L1 :|: L2 :|: *)
+    (* f_div_loc :|: *)
+    (* f_group_one_loc :|: *)
+    (* f_prod_loc :|: *)
+    (* f_g_pow_loc :|: *)
+    (* f_g_loc :|: f_hash_loc :|: f_mul_loc :|: f_random_field_elem_loc :|: f_sub_loc :|: *)
+    (* f_pow_loc :|: *)
+    (* f_field_one_loc :|: *)
+    (* f_field_zero_loc :|: fset [cast_vote_state_ret_loc (n := n);prod1_loc (n := n);prod2_loc (n := n)] (* :|: f_get_loc :|: f_clone_loc :|: f_accept_loc :|: f_parameter_cursor_loc *)) (I1 :|: I2) ((t_OvnContractState (n := n))) *) in
     solve_lift ret_both tt (* assign body todo(term) *) : both (L1 :|: L2 :|:
-     fset [cast_vote_state_ret_loc;prod1_loc;prod2_loc] :|: Hacspec_ovn_Ovn_traits.f_div_loc :|:
-    Hacspec_ovn_Ovn_traits.f_group_one_loc :|:
-    Hacspec_ovn_Ovn_traits.f_prod_loc :|:
-    Hacspec_ovn_Ovn_traits.f_g_pow_loc :|:
-    Hacspec_ovn_Ovn_traits.f_pow_loc :|:
-    Hacspec_ovn_Ovn_traits.f_field_one_loc :|:
-    Hacspec_ovn_Ovn_traits.f_field_zero_loc (* :|: f_get_loc :|: f_clone_loc :|: f_accept_loc :|: f_parameter_cursor_loc *)) _ _ in
-    letb _ := letb cast_vote_state_ret loc(cast_vote_state_ret_loc) := Build_t_OvnContractState[cast_vote_state_ret] (f_zkp_vis := update_at_usize (f_zkp_vis cast_vote_state_ret) (cast_int (WS2 := U32) (f_cvp_i params)) zkp_vi) in
+    f_div_loc :|:
+    f_group_one_loc :|:
+    f_prod_loc :|:
+    f_g_pow_loc :|:
+    f_g_loc :|: f_hash_loc :|: f_mul_loc :|: f_random_field_elem_loc :|: f_sub_loc :|:
+    f_pow_loc :|:
+    f_field_one_loc :|:
+    f_field_zero_loc :|:
+    fset [cast_vote_state_ret_loc (n := n);prod1_loc;prod2_loc] (* :|: f_get_loc :|: f_clone_loc :|: f_accept_loc :|: f_parameter_cursor_loc *)) _ _ in
+    letb _ := letb cast_vote_state_ret loc(cast_vote_state_ret_loc (n := n)) := Build_t_OvnContractState[cast_vote_state_ret] (f_zkp_vis := update_at_usize (f_zkp_vis cast_vote_state_ret) (cast_int (WS2 := U32) (f_cvp_i params)) zkp_vi)(* : both (L1 :|: L2 :|: *)
+    (* f_div_loc :|: *)
+    (* f_group_one_loc :|: *)
+    (* f_prod_loc :|: *)
+    (* f_g_pow_loc :|: *)
+    (* f_g_loc :|: f_hash_loc :|: f_mul_loc :|: f_random_field_elem_loc :|: f_sub_loc :|: *)
+    (* f_pow_loc :|: *)
+    (* f_field_one_loc :|: *)
+    (* f_field_zero_loc :|: fset [cast_vote_state_ret_loc (n := n);prod1_loc (n := n);prod2_loc (n := n)] (* :|: f_get_loc :|: f_clone_loc :|: f_accept_loc :|: f_parameter_cursor_loc *)) (I1 :|: I2) (t_OvnContractState (n := n)) *) in
     solve_lift ret_both tt (* assign body todo(term) *) : both (L1 :|: L2 :|:
-    fset [cast_vote_state_ret_loc;prod1_loc;prod2_loc] :|: Hacspec_ovn_Ovn_traits.f_div_loc :|:
-    Hacspec_ovn_Ovn_traits.f_group_one_loc :|:
-    Hacspec_ovn_Ovn_traits.f_prod_loc :|:
-    Hacspec_ovn_Ovn_traits.f_g_pow_loc :|:
-    Hacspec_ovn_Ovn_traits.f_pow_loc :|:
-    Hacspec_ovn_Ovn_traits.f_field_one_loc :|:
-    Hacspec_ovn_Ovn_traits.f_field_zero_loc (* :|: f_get_loc :|: f_clone_loc :|: f_accept_loc :|: f_parameter_cursor_loc *)) _ _ in
-    Result_Ok (prod_b (f_accept (* (ret_both (tt : 'unit)) *),cast_vote_state_ret))))) : both (L1 :|: L2 :|:
-    fset [cast_vote_state_ret_loc;prod1_loc;prod2_loc] :|: Hacspec_ovn_Ovn_traits.f_div_loc :|:
-    Hacspec_ovn_Ovn_traits.f_group_one_loc :|:
-    Hacspec_ovn_Ovn_traits.f_prod_loc :|:
-    Hacspec_ovn_Ovn_traits.f_g_pow_loc :|:
-    Hacspec_ovn_Ovn_traits.f_pow_loc :|:
-    Hacspec_ovn_Ovn_traits.f_field_one_loc :|:
-    Hacspec_ovn_Ovn_traits.f_field_zero_loc (* :|: f_get_loc :|: f_clone_loc :|: f_accept_loc :|: f_parameter_cursor_loc *)) (I1 :|: I2) (t_Result ((v_A × t_OvnContractState (v_Z := v_Z) (v_G := v_G) (n := n) (* (both (fset []) (fset []) (uint_size)) *))) (t_ParseError)).
+    f_div_loc :|:
+    f_group_one_loc :|:
+    f_prod_loc :|:
+    f_g_pow_loc :|:
+    f_g_loc :|: f_hash_loc :|: f_mul_loc :|: f_random_field_elem_loc :|: f_sub_loc :|:
+    f_pow_loc :|:
+    f_field_one_loc :|:
+    f_field_zero_loc :|:
+    fset [cast_vote_state_ret_loc (n := n);prod1_loc;prod2_loc] (* :|: f_get_loc :|: f_clone_loc :|: f_accept_loc :|: f_parameter_cursor_loc *)) _ _ in
+    Result_Ok (prod_b (f_accept (* (ret_both (tt : 'unit)) *),cast_vote_state_ret))))) : both (L1 :|: L2 :|: f_div_loc :|:
+    f_group_one_loc :|:
+    f_prod_loc :|:
+    f_g_pow_loc :|:
+    f_g_loc :|: f_hash_loc :|: f_mul_loc :|: f_random_field_elem_loc :|: f_sub_loc :|:
+    f_pow_loc :|:
+    f_field_one_loc :|:
+    f_field_zero_loc :|:
+    fset [cast_vote_state_ret_loc (n := n);prod1_loc;prod2_loc] (* :|: f_get_loc :|: f_clone_loc :|: f_accept_loc :|: f_parameter_cursor_loc *)) (I1 :|: I2) (t_Result ((v_A × t_OvnContractState (v_Z := v_Z) (v_G := v_G) (n := n) (* (both (fset []) (fset []) (uint_size)) *))) (t_ParseError)).
 Next Obligation.
   intros.
-  autounfold.
+  simpl.
+  unfold cast_vote_obligations_obligation_1.
+  unfold cast_vote_obligations_obligation_7.
   solve_ssprove_obligations.
 Qed.
 Next Obligation.
+  intros.
+  simpl.
+  unfold cast_vote_obligations_obligation_2.
+  unfold cast_vote_obligations_obligation_9.
   solve_ssprove_obligations.
 Qed.
 Next Obligation.
+  intros.
+  simpl.
+  unfold cast_vote_obligations_obligation_7.
+solve_ssprove_obligations.
+Qed.
+Next Obligation.
+  intros.
+  simpl.
+  unfold cast_vote_obligations_obligation_9.
   solve_ssprove_obligations.
 Qed.
 Next Obligation.
+  intros.
+  simpl.
+  unfold cast_vote_obligations_obligation_3.
+  unfold cast_vote_obligations_obligation_5.
   solve_ssprove_obligations.
 Qed.
 Next Obligation.
+  intros.
+  simpl.
+  unfold cast_vote_obligations_obligation_4.
+  unfold cast_vote_obligations_obligation_6.
   solve_ssprove_obligations.
 Qed.
 Next Obligation.
+  intros.
+  simpl.
+  unfold cast_vote_obligations_obligation_3.
+  unfold cast_vote_obligations_obligation_5.
   solve_ssprove_obligations.
 Qed.
 Next Obligation.
+  intros.
+  simpl.
+  unfold cast_vote_obligations_obligation_4.
+  unfold cast_vote_obligations_obligation_6.
   solve_ssprove_obligations.
 Qed.
 Next Obligation.
+  intros.
+  simpl.
+  unfold cast_vote_obligations_obligation_1.
+  unfold cast_vote_obligations_obligation_5.
   solve_ssprove_obligations.
 Qed.
 Next Obligation.
-  refine (solve_lift ret_both 0).
-  solve_ssprove_obligations.
-  rewrite fset0E.
+  intros.
+  simpl.
+  unfold cast_vote_obligations_obligation_2.
+  unfold cast_vote_obligations_obligation_6.
   solve_ssprove_obligations.
 Qed.
 Next Obligation.
@@ -559,147 +618,252 @@ Next Obligation.
   unfold cast_vote_obligations_obligation_5.
   destruct H5.
   destruct H4.
-  split_fsubset_lhs.
-  now solve_single_fset_fsubset.
-  solve_single_fset_fsubset.
-  solve_single_fset_fsubset.
-  solve_single_fset_fsubset.
-  solve_single_fset_fsubset.
-  solve_single_fset_fsubset.
-  solve_single_fset_fsubset.
-  solve_single_fset_fsubset.
-  solve_single_fset_fsubset.
-  solve_single_fset_fsubset.
-  solve_single_fset_fsubset.
-  solve_single_fset_fsubset.
-  solve_single_fset_fsubset.
-  solve_single_fset_fsubset.
-  solve_single_fset_fsubset.
-  solve_single_fset_fsubset.
-  solve_single_fset_fsubset.
-  solve_single_fset_fsubset.
-  solve_single_fset_fsubset.
-  solve_single_fset_fsubset.
-  solve_single_fset_fsubset.
-  solve_single_fset_fsubset.
-  solve_single_fset_fsubset.
-  solve_single_fset_fsubset.
-  solve_single_fset_fsubset.
-  solve_single_fset_fsubset.
-  solve_single_fset_fsubset.
-  solve_single_fset_fsubset.
-  solve_single_fset_fsubset.
+  solve_ssprove_obligations.
 Qed.
-
-Solve All Obligations with solve_ssprove_obligations.
-Admit Obligations. (* TODO: fix *)
+Next Obligation.
+  simpl.
+  intros.
+  unfold cast_vote_obligations_obligation_6.
+  unfold cast_vote_obligations_obligation_27.
+  solve_ssprove_obligations.
+Qed.
+Solve All Obligations with timeout 2 ( solve_ssprove_obligations ; ((now (rewrite !fset0E ; apply (ret_both 0))) || (now destruct from_uint_size))).
+Next Obligation.
+    simpl.
+  intros.
+  unfold cast_vote_obligations_obligation_5.
+  unfold cast_vote_obligations_obligation_27.
+  normalize_fset.
+  destruct H5.
+  destruct H4.
+  solve_ssprove_obligations.
+Qed.
+Next Obligation.
+  simpl.
+  intros.
+  unfold cast_vote_obligations_obligation_6.
+  unfold cast_vote_obligations_obligation_33.
+  destruct H5.
+  destruct H4.
+  solve_ssprove_obligations.
+Qed.
+Next Obligation.
+  simpl.
+  intros.
+  unfold cast_vote_obligations_obligation_7.
+  destruct H5.
+  destruct H4.
+  normalize_fset.
+  split_fsubset_lhs ; admit. (* Somethings wrong *)
+Admitted.
+Next Obligation.
+  simpl.
+  intros.
+  unfold cast_vote_obligations_obligation_33.
+  unfold cast_vote_obligations_obligation_9.
+  solve_ssprove_obligations.
+Qed.
+Next Obligation.
+  simpl.
+  intros.
+  unfold cast_vote_obligations_obligation_7.
+  admit. (* Somethings wrong *)
+Admitted.
+Next Obligation.
+  simpl.
+  intros.
+  unfold cast_vote_obligations_obligation_27.
+  unfold cast_vote_obligations_obligation_9.
+  solve_ssprove_obligations.
+Qed.
+Next Obligation.
+  simpl.
+  intros.
+  unfold cast_vote_obligations_obligation_5.
+  unfold cast_vote_obligations_obligation_7.
+  admit. (* Somethings wrong *)
+Admitted.
+Next Obligation.
+  simpl.
+  intros.
+  unfold cast_vote_obligations_obligation_27.
+  unfold cast_vote_obligations_obligation_9.
+  unfold cast_vote_obligations_obligation_6.
+  solve_ssprove_obligations.
+Qed.
+Next Obligation.
+  simpl.
+  intros.
+  unfold cast_vote_obligations_obligation_5.
+  unfold cast_vote_obligations_obligation_7.
+  admit. (* Somethings wrong *)
+Admitted.
+Next Obligation.
+  simpl.
+  intros.
+  unfold cast_vote_obligations_obligation_27.
+  unfold cast_vote_obligations_obligation_9.
+  unfold cast_vote_obligations_obligation_6.
+  solve_ssprove_obligations.
+Qed.
+Next Obligation.
+  simpl.
+  intros.
+  unfold cast_vote_obligations_obligation_5.
+  unfold cast_vote_obligations_obligation_7.
+  admit. (* Somethings wrong *)
+Admitted.
+Next Obligation.
+  simpl.
+  intros.
+  unfold cast_vote_obligations_obligation_27.
+  unfold cast_vote_obligations_obligation_9.
+  unfold cast_vote_obligations_obligation_6.
+  solve_ssprove_obligations.
+Qed.
+Next Obligation.
+  simpl.
+  intros.
+  unfold cast_vote_obligations_obligation_5.
+  unfold cast_vote_obligations_obligation_7.
+  solve_ssprove_obligations.
+Qed.
+Next Obligation.
+  simpl.
+  intros.
+  unfold cast_vote_obligations_obligation_27.
+  unfold cast_vote_obligations_obligation_9.
+  unfold cast_vote_obligations_obligation_6.
+  solve_ssprove_obligations.
+Qed.
+Next Obligation.
+  simpl.
+  intros.
+  unfold cast_vote_obligations_obligation_5.
+  unfold cast_vote_obligations_obligation_7.
+  solve_ssprove_obligations.
+Qed.
+Next Obligation.
+  simpl.
+  intros.
+  solve_ssprove_obligations.
+Qed.
+Next Obligation.
+  simpl.
+  intros.
+  solve_ssprove_obligations.
+Qed.
+Next Obligation.
+  simpl.
+  intros.
+  solve_ssprove_obligations.
+Qed.
 Fail Next Obligation.
-Obligation Tactic := (* try timeout 2 *) solve_ssprove_obligations.
 
-Definition commit_to_vote_state_ret_loc {v_Z : _} {v_G : _} {n : both (fset []) (fset []) (uint_size)} {v_A : _} {impl_574521470_ : _} `{ t_Sized (v_Z)} `{ t_Sized (v_G)} `{ t_Sized (v_A)} `{ t_Sized (impl_574521470_)} `{ t_Z_Field (v_Z)} `{ t_Group (v_G) (v_Z)} `{ t_HasActions (v_A)} `{ t_HasReceiveContext (impl_574521470_) ('unit)} : Location :=
-  (t_OvnContractState (v_Z := v_Z) (v_G := v_G) (n := n)(* (both (fset []) (fset []) (uint_size)) *);3%nat).
-Equations commit_to_vote {L1 : {fset Location}} {L2 : {fset Location}} {I1 : Interface} {I2 : Interface} {v_Z : _} {v_G : _} {n : both (fset []) (fset []) (uint_size)} {v_A : _} {impl_574521470_ : _} `{ t_Sized (v_Z)} `{ t_Sized (v_G)} `{ t_Sized (v_A)} `{ t_Sized (impl_574521470_)} `{ t_Z_Field (v_Z)} `{ t_Group (v_G) (v_Z)} `{ t_HasActions (v_A)} `{ t_HasReceiveContext (impl_574521470_) ('unit)} (ctx : both L1 I1 (impl_574521470_)) (state : both L2 I2 (t_OvnContractState (v_Z := v_Z) (v_G := v_G) (n := n)(* (both (fset []) (fset []) (uint_size)) *))) : both (L1 :|: L2 :|: fset [commit_to_vote_state_ret_loc (n := n);prod1_loc (n := n);prod2_loc (n := n)] (* :|: f_get_loc :|: f_clone_loc :|: f_into_iter_loc :|: f_end_loc :|: f_start_loc :|: f_accept_loc :|: f_parameter_cursor_loc *)) (I1 :|: I2) (t_Result ((v_A × t_OvnContractState (v_Z := v_Z) (v_G := v_G) (n := n)(* (both (fset []) (fset []) (uint_size)) *))) (t_ParseError)) :=
-  commit_to_vote ctx state  :=
-    solve_lift (run (letb '(_,out) := f_get (f_parameter_cursor ctx) in
-    letm[choice_typeMonad.result_bind_code (t_Result ((v_A × t_OvnContractState (v_Z := v_Z) (v_G := v_G) (n := n)(* (both (fset []) (fset []) (uint_size)) *))) (t_ParseError))] (params : t_CastVoteParam (v_Z)) := matchb out with
-    | Result_Ok_case x =>
-      letb x := ret_both ((x) (* : (t_CastVoteParam (v_Z)) *)) in
-      ControlFlow_Continue (solve_lift x)
-    | Result_Err_case x =>
-      letb x := ret_both ((x) : (t_ParseError)) in
-      letm[choice_typeMonad.result_bind_code (t_Result ((v_A × t_OvnContractState (v_Z := v_Z) (v_G := v_G) (n := n)(* (both (fset []) (fset []) (uint_size)) *))) (t_ParseError))] hoist3 := v_Break (Result_Err _ (* ParseError *)) in
-      ControlFlow_Continue (solve_lift (never_to_any hoist3))
-    end in
-    ControlFlow_Continue (letb _ := foldi_both_list (f_into_iter (Build_t_Range (f_start := ret_both (0 : uint_size)) (f_end := n))) (fun i =>
-      ssp (fun _ =>
-        solve_lift (ifb (* not *) negb (schnorr_zkp_validate ((f_g_pow_xis state).a[i]) ((f_zkp_xis state).a[i]))
-        then letm[choice_typeMonad.result_bind_code (t_Result ((v_A × t_OvnContractState (v_Z := v_Z) (v_G := v_G) (n := n)(* (both (fset []) (fset []) (uint_size)) *))) (t_ParseError))] hoist4 := v_Break (Result_Err _ (* ParseError *)) in
-        ControlFlow_Continue (never_to_any hoist4)
-        else Result_Ok (solve_lift ret_both tt)) : both (*0*)(L2:|:fset []) (I2) (* ((* t_ControlFlow *) t_Result (t_Result ((v_A × t_OvnContractState (v_Z := v_Z) (v_G := v_G) (n := n)(* (both (fset []) (fset []) (uint_size)) *))) (t_ParseError)) ('unit)) *) _)) (Result_Ok (solve_lift ret_both (tt : 'unit))) in
-    letb g_pow_yi := compute_g_pow_yi (cast_int (WS2 := U32) (f_cvp_i params)) (f_g_pow_xis state) in
-    letb g_pow_xi_yi_vi := compute_group_element_for_vote (f_cvp_xi params) (f_cvp_vote params) g_pow_yi in
-    letb commit_vi := commit_to g_pow_xi_yi_vi in
-    letb commit_to_vote_state_ret loc(commit_to_vote_state_ret_loc) := f_clone state in
-    letb _ := letb commit_to_vote_state_ret loc(commit_to_vote_state_ret_loc) := Build_t_OvnContractState[commit_to_vote_state_ret] (f_commit_vis := update_at_usize (f_commit_vis commit_to_vote_state_ret) (cast_int (WS2 := U32) (f_cvp_i params)) commit_vi) in
-    solve_lift ret_both tt (* assign body todo(term) *) in
-    Result_Ok (prod_b (f_accept (* (ret_both (tt : 'unit)) *),commit_to_vote_state_ret))))) : both (L1 :|: L2 :|: fset [commit_to_vote_state_ret_loc;prod1_loc;prod2_loc] (* :|: f_get_loc :|: f_clone_loc :|: f_into_iter_loc :|: f_end_loc :|: f_start_loc :|: f_accept_loc :|: f_parameter_cursor_loc *)) (I1 :|: I2) (t_Result ((v_A × t_OvnContractState (v_Z := v_Z) (v_G := v_G) (n := n)(* (both (fset []) (fset []) (uint_size)) *))) (t_ParseError)).
-Admit Obligations.
-Fail Next Obligation.
-
-Equations init_ovn_contract {L1 : {fset Location}} {I1 : Interface} {v_Z : _} {v_G : _} {n : both (fset []) (fset []) (uint_size)} `{ t_Sized (v_Z)} `{ t_Sized (v_G)} `{ t_Z_Field (v_Z)} `{ t_Group (v_G) (v_Z)} (_ : both L1 I1 ('unit)) : both (L1 (* :|: f_or_zkp_a1_loc :|: f_or_zkp_a2_loc :|: f_or_zkp_b1_loc :|: f_or_zkp_b2_loc :|: f_or_zkp_c_loc :|: f_or_zkp_d1_loc :|: f_or_zkp_d2_loc :|: f_or_zkp_r1_loc :|: f_or_zkp_r2_loc :|: f_or_zkp_x_loc :|: f_or_zkp_y_loc :|: f_commit_vis_loc :|: f_g_pow_xi_yi_vis_loc :|: f_g_pow_xis_loc :|: f_tally_loc :|: f_zkp_vis_loc :|: f_zkp_xis_loc :|: f_schnorr_zkp_c_loc :|: f_schnorr_zkp_u_loc :|: f_schnorr_zkp_z_loc *) :|: f_group_one_loc :|: f_field_zero_loc) I1 (t_Result (t_OvnContractState (v_Z := v_Z) (v_G := v_G) (n := n)(* (both (fset []) (fset []) (uint_size)) *)) (t_Reject)) :=
-  init_ovn_contract _  :=
-    Result_Ok (solve_lift (Build_t_OvnContractState (f_g_pow_xis := repeat (f_group_one (ret_both (tt : 'unit))) n) (f_zkp_xis := repeat (Build_t_SchnorrZKPCommit (f_schnorr_zkp_u := f_group_one (ret_both (tt : 'unit))) (f_schnorr_zkp_z := f_field_zero (ret_both (tt : 'unit))) (f_schnorr_zkp_c := f_field_zero (ret_both (tt : 'unit)))) n) (f_commit_vis := repeat (f_field_zero (ret_both (tt : 'unit))) n) (f_g_pow_xi_yi_vis := repeat (f_group_one (ret_both (tt : 'unit))) n) (f_zkp_vis := repeat (Build_t_OrZKPCommit (f_or_zkp_x := f_group_one (ret_both (tt : 'unit))) (f_or_zkp_y := f_group_one (ret_both (tt : 'unit))) (f_or_zkp_a1 := f_group_one (ret_both (tt : 'unit))) (f_or_zkp_b1 := f_group_one (ret_both (tt : 'unit))) (f_or_zkp_a2 := f_group_one (ret_both (tt : 'unit))) (f_or_zkp_b2 := f_group_one (ret_both (tt : 'unit))) (f_or_zkp_c := f_field_zero (ret_both (tt : 'unit))) (f_or_zkp_d1 := f_field_zero (ret_both (tt : 'unit))) (f_or_zkp_d2 := f_field_zero (ret_both (tt : 'unit))) (f_or_zkp_r1 := f_field_zero (ret_both (tt : 'unit))) (f_or_zkp_r2 := f_field_zero (ret_both (tt : 'unit)))) n) (f_tally := ret_both (0 : int32)))) : both (L1 (* :|: f_or_zkp_a1_loc :|: f_or_zkp_a2_loc :|: f_or_zkp_b1_loc :|: f_or_zkp_b2_loc :|: f_or_zkp_c_loc :|: f_or_zkp_d1_loc :|: f_or_zkp_d2_loc :|: f_or_zkp_r1_loc :|: f_or_zkp_r2_loc :|: f_or_zkp_x_loc :|: f_or_zkp_y_loc :|: f_commit_vis_loc :|: f_g_pow_xi_yi_vis_loc :|: f_g_pow_xis_loc :|: f_tally_loc :|: f_zkp_vis_loc :|: f_zkp_xis_loc :|: f_schnorr_zkp_c_loc :|: f_schnorr_zkp_u_loc :|: f_schnorr_zkp_z_loc *) :|: f_group_one_loc :|: f_field_zero_loc) I1 (t_Result (t_OvnContractState (v_Z := v_Z) (v_G := v_G) (n := n)(* (both (fset []) (fset []) (uint_size)) *)) (t_Reject)).
-Fail Next Obligation.
-
-Definition register_vote_state_ret_loc {v_Z : _} {v_G : _} {n : both (fset []) (fset []) (uint_size)} {v_A : _} {impl_574521470_ : _} `{ t_Sized (v_Z)} `{ t_Sized (v_G)} `{ t_Sized (v_A)} `{ t_Sized (impl_574521470_)} `{ t_Z_Field (v_Z)} `{ t_Group (v_G) (v_Z)} `{ t_HasActions (v_A)} `{ t_HasReceiveContext (impl_574521470_) ('unit)} : Location :=
-  (t_OvnContractState (v_Z := v_Z) (v_G := v_G) (n := n)(* (both (fset []) (fset []) (uint_size)) *);4%nat).
-Equations register_vote {L1 : {fset Location}} {L2 : {fset Location}} {I1 : Interface} {I2 : Interface} {v_Z : _} {v_G : _} {n : both (fset []) (fset []) (uint_size)} {v_A : _} {impl_574521470_ : _} `{ t_Sized (v_Z)} `{ t_Sized (v_G)} `{ t_Sized (v_A)} `{ t_Sized (impl_574521470_)} `{ t_Z_Field (v_Z)} `{ t_Group (v_G) (v_Z)} `{ t_HasActions (v_A)} `{ t_HasReceiveContext (impl_574521470_) ('unit)} (ctx : both L1 I1 (impl_574521470_)) (state : both L2 I2 (t_OvnContractState (v_Z := v_Z) (v_G := v_G) (n := n)(* (both (fset []) (fset []) (uint_size)) *))) : both (L1 :|: L2 :|: fset [register_vote_state_ret_loc (n := n)] (* :|: f_get_loc :|: f_clone_loc :|: f_accept_loc :|: f_parameter_cursor_loc *) :|: f_g_pow_loc) (I1 :|: I2) (t_Result ((v_A × t_OvnContractState (v_Z := v_Z) (v_G := v_G) (n := n)(* (both (fset []) (fset []) (uint_size)) *))) (t_ParseError)) :=
-  register_vote ctx state  :=
-    solve_lift (run (letb '(_,out) := f_get (f_parameter_cursor ctx) in
-    letm[choice_typeMonad.result_bind_code (t_Result ((v_A × t_OvnContractState (v_Z := v_Z) (v_G := v_G) (n := n)(* (both (fset []) (fset []) (uint_size)) *))) (t_ParseError))] (params : t_RegisterParam (v_Z)) := matchb out with
-    | Result_Ok_case x =>
-      letb x := ret_both ((x) (* : (t_RegisterParam (v_Z)) *)) in
-      ControlFlow_Continue (solve_lift x)
-    | Result_Err_case x =>
-      letb x := ret_both ((x) : (t_ParseError)) in
-      letm[choice_typeMonad.result_bind_code (t_Result ((v_A × t_OvnContractState (v_Z := v_Z) (v_G := v_G) (n := n)(* (both (fset []) (fset []) (uint_size)) *))) (t_ParseError))] hoist5 := v_Break (Result_Err (* ParseError *) _) in
-      ControlFlow_Continue (solve_lift (never_to_any hoist5))
-    end in
-    ControlFlow_Continue (letb g_pow_xi := f_g_pow (f_rp_xi params) in
-    letb zkp_xi := schnorr_zkp (f_rp_zkp_random params) g_pow_xi (f_rp_xi params) in
-    letb register_vote_state_ret loc(register_vote_state_ret_loc) := f_clone state in
-    letb _ := letb register_vote_state_ret loc(register_vote_state_ret_loc) := Build_t_OvnContractState[register_vote_state_ret] (f_g_pow_xis := update_at_usize (f_g_pow_xis register_vote_state_ret) (cast_int (WS2 := U32) (f_rp_i params)) g_pow_xi) in
-    solve_lift ret_both tt (* assign body todo(term) *) in
-    letb _ := letb register_vote_state_ret loc(register_vote_state_ret_loc) := Build_t_OvnContractState[register_vote_state_ret] (f_zkp_xis := update_at_usize (f_zkp_xis register_vote_state_ret) (cast_int (WS2 := U32) (f_rp_i params)) zkp_xi) in
-    solve_lift ret_both tt (* assign body todo(term) *) in
-                              Result_Ok (prod_b (f_accept (* (ret_both (tt : 'unit)) *),register_vote_state_ret))))) : both (L1 :|: L2 :|: fset [register_vote_state_ret_loc (n := n)] (* :|: f_get_loc :|: f_clone_loc :|: f_accept_loc :|: f_parameter_cursor_loc *) :|: f_g_pow_loc) (I1 :|: I2) (t_Result ((v_A × t_OvnContractState (v_Z := v_Z) (v_G := v_G) (n := n)(* (both (fset []) (fset []) (uint_size)) *))) (t_ParseError)).
-Admit Obligations.
-Fail Next Obligation.
-
-Definition curr_loc {v_Z : _} {v_G : _} {n : both (fset []) (fset []) (uint_size)} {v_A : _} {impl_574521470_ : _} `{ t_Sized (v_Z)} `{ t_Sized (v_G)} `{ t_Sized (v_A)} `{ t_Sized (impl_574521470_)} `{ t_Z_Field (v_Z)} `{ t_Group (v_G) (v_Z)} `{ t_HasActions (v_A)} `{ t_HasReceiveContext (impl_574521470_) ('unit)} : Location :=
-  (f_field_type;5%nat).
-Definition tally_loc {v_Z : _} {v_G : _} {n : both (fset []) (fset []) (uint_size)} {v_A : _} {impl_574521470_ : _} `{ t_Sized (v_Z)} `{ t_Sized (v_G)} `{ t_Sized (v_A)} `{ t_Sized (impl_574521470_)} `{ t_Z_Field (v_Z)} `{ t_Group (v_G) (v_Z)} `{ t_HasActions (v_A)} `{ t_HasReceiveContext (impl_574521470_) ('unit)} : Location :=
-  (int32;6%nat).
-Definition tally_votes_state_ret_loc {v_Z : _} {v_G : _} {n : both (fset []) (fset []) (uint_size)} {v_A : _} {impl_574521470_ : _} `{ t_Sized (v_Z)} `{ t_Sized (v_G)} `{ t_Sized (v_A)} `{ t_Sized (impl_574521470_)} `{ t_Z_Field (v_Z)} `{ t_Group (v_G) (v_Z)} `{ t_HasActions (v_A)} `{ t_HasReceiveContext (impl_574521470_) ('unit)} : Location :=
-  (t_OvnContractState (v_Z := v_Z) (v_G := v_G) (n := n)(* (both (fset []) (fset []) (uint_size)) *);7%nat).
-Definition vote_result_loc {v_Z : _} {v_G : _} {n : both (fset []) (fset []) (uint_size)} {v_A : _} {impl_574521470_ : _} `{ t_Sized (v_Z)} `{ t_Sized (v_G)} `{ t_Sized (v_A)} `{ t_Sized (impl_574521470_)} `{ t_Z_Field (v_Z)} `{ t_Group (v_G) (v_Z)} `{ t_HasActions (v_A)} `{ t_HasReceiveContext (impl_574521470_) ('unit)} : Location :=
-  (f_group_type;8%nat).
-(* Equations tally_votes {L1 : {fset Location}} {L2 : {fset Location}} {I1 : Interface} {I2 : Interface} {v_Z : _} {v_G : _} {n : both (fset []) (fset []) (uint_size)} {v_A : _} {impl_574521470_ : _} `{ t_Sized (v_Z)} `{ t_Sized (v_G)} `{ t_Sized (v_A)} `{ t_Sized (impl_574521470_)} `{ t_Z_Field (v_Z)} `{ t_Group (v_G) (v_Z)} `{ t_HasActions (v_A)} `{ t_HasReceiveContext (impl_574521470_) ('unit)} (_ : both L1 I1 (impl_574521470_)) (state : both L2 I2 (t_OvnContractState (v_Z := v_Z) (v_G := v_G) (n := n)(* (both (fset []) (fset []) (uint_size)) *))) : both (L1 :|: L2 :|: fset [curr_loc (n := n);tally_loc (n := n);tally_votes_state_ret_loc (n := n);vote_result_loc (n := n);prod1_loc (n := n);prod2_loc (n := n)] (* :|: f_clone_loc :|: f_eq_loc :|: f_into_iter_loc :|: f_end_loc :|: f_start_loc :|: f_accept_loc *) :|: f_g_pow_loc :|: f_group_one_loc :|: f_prod_loc :|: f_add_loc :|: f_field_one_loc :|: f_field_zero_loc) (I1 :|: I2) (t_Result ((v_A × t_OvnContractState (v_Z := v_Z) (v_G := v_G) (n := n)(* (both (fset []) (fset []) (uint_size)) *))) (t_ParseError)) := *)
-(*   tally_votes _ state  := *)
-(*     letb _ := foldi_both_list (f_into_iter (Build_t_Range (f_start := ret_both (0 : uint_size)) (f_end := n))) (fun i => *)
+(* Definition commit_to_vote_state_ret_loc {v_Z : _} {v_G : _} {n : both (fset []) (fset []) (uint_size)} {v_A : _} {impl_574521470_ : _} `{ t_Sized (v_Z)} `{ t_Sized (v_G)} `{ t_Sized (v_A)} `{ t_Sized (impl_574521470_)} `{ t_Z_Field (v_Z)} `{ t_Group (v_G) (v_Z)} `{ t_HasActions (v_A)} `{ t_HasReceiveContext (impl_574521470_) ('unit)} : Location := *)
+(*   (t_OvnContractState (v_Z := v_Z) (v_G := v_G) (n := n)(* (both (fset []) (fset []) (uint_size)) *);3%nat). *)
+(* Equations commit_to_vote {L1 : {fset Location}} {L2 : {fset Location}} {I1 : Interface} {I2 : Interface} {v_Z : _} {v_G : _} {n : both (fset []) (fset []) (uint_size)} {v_A : _} {impl_574521470_ : _} `{ t_Sized (v_Z)} `{ t_Sized (v_G)} `{ t_Sized (v_A)} `{ t_Sized (impl_574521470_)} `{ t_Z_Field (v_Z)} `{ t_Group (v_G) (v_Z)} `{ t_HasActions (v_A)} `{ t_HasReceiveContext (impl_574521470_) ('unit)} (ctx : both L1 I1 (impl_574521470_)) (state : both L2 I2 (t_OvnContractState (v_Z := v_Z) (v_G := v_G) (n := n)(* (both (fset []) (fset []) (uint_size)) *))) : both (L1 :|: L2 :|: fset [commit_to_vote_state_ret_loc (n := n);prod1_loc (n := n);prod2_loc (n := n)] (* :|: f_get_loc :|: f_clone_loc :|: f_into_iter_loc :|: f_end_loc :|: f_start_loc :|: f_accept_loc :|: f_parameter_cursor_loc *)) (I1 :|: I2) (t_Result ((v_A × t_OvnContractState (v_Z := v_Z) (v_G := v_G) (n := n)(* (both (fset []) (fset []) (uint_size)) *))) (t_ParseError)) := *)
+(*   commit_to_vote ctx state  := *)
+(*     solve_lift (run (letb '(_,out) := f_get (f_parameter_cursor ctx) in *)
+(*     letm[choice_typeMonad.result_bind_code (t_Result ((v_A × t_OvnContractState (v_Z := v_Z) (v_G := v_G) (n := n)(* (both (fset []) (fset []) (uint_size)) *))) (t_ParseError))] (params : t_CastVoteParam (v_Z)) := matchb out with *)
+(*     | Result_Ok_case x => *)
+(*       letb x := ret_both ((x) (* : (t_CastVoteParam (v_Z)) *)) in *)
+(*       ControlFlow_Continue (solve_lift x) *)
+(*     | Result_Err_case x => *)
+(*       letb x := ret_both ((x) : (t_ParseError)) in *)
+(*       letm[choice_typeMonad.result_bind_code (t_Result ((v_A × t_OvnContractState (v_Z := v_Z) (v_G := v_G) (n := n)(* (both (fset []) (fset []) (uint_size)) *))) (t_ParseError))] hoist3 := v_Break (Result_Err _ (* ParseError *)) in *)
+(*       ControlFlow_Continue (solve_lift (never_to_any hoist3)) *)
+(*     end in *)
+(*     ControlFlow_Continue (letb _ := foldi_both_list (f_into_iter (Build_t_Range (f_start := ret_both (0 : uint_size)) (f_end := n))) (fun i => *)
 (*       ssp (fun _ => *)
-(*         letb g_pow_yi := compute_g_pow_yi i (f_g_pow_xis state) in *)
-(*         letm[choice_typeMonad.result_bind_code (t_Result ((v_A × t_OvnContractState (v_Z := v_Z) (v_G := v_G) (n := n)(* (both (fset []) (fset []) (uint_size)) *))) (t_ParseError))] _ := ControlFlow_Continue (ifb (* not *)negb (zkp_one_out_of_two_validate g_pow_yi ((f_zkp_vis state).a[i])) *)
-(*         then letm[choice_typeMonad.result_bind_code (t_Result ((v_A × t_OvnContractState (v_Z := v_Z) (v_G := v_G) (n := n)(* (both (fset []) (fset []) (uint_size)) *))) (t_ParseError))] hoist6 := v_Break (Result_Err _ (* ParseError *)) in *)
-(*         ControlFlow_Continue (never_to_any hoist6) *)
-(*         else Result_Ok (solve_lift ret_both tt)) in *)
-(*         solve_lift (ifb (* not *)negb (check_commitment ((f_g_pow_xi_yi_vis state).a[i]) ((f_commit_vis state).a[i])) *)
-(*         then letm[choice_typeMonad.result_bind_code (t_Result ((v_A × t_OvnContractState (v_Z := v_Z) (v_G := v_G) (n := n)(* (both (fset []) (fset []) (uint_size)) *))) (t_ParseError))] hoist7 := v_Break (Result_Err (* ParseError *) _) in *)
-(*         ControlFlow_Continue (never_to_any hoist7) *)
-(*         else Result_Ok (solve_lift ret_both tt)) : both (*0*)(L2:|:fset []) (I2) _ (* (t_ControlFlow (t_Result ((v_A × t_OvnContractState (v_Z := v_Z) (v_G := v_G) (n := n)(* (both (fset []) (fset []) (uint_size)) *))) (t_ParseError)) ('unit)) *))) (Result_Ok (ret_both (tt : 'unit))) in *)
-(*     letb vote_result loc(vote_result_loc) := f_group_one (ret_both (tt : 'unit)) in *)
-(*     letb _ := foldi_both_list (f_into_iter (f_g_pow_xi_yi_vis state)) (fun g_pow_vote => *)
-(*       ssp (fun _ => *)
-(*         letb vote_result loc(vote_result_loc) := f_prod vote_result g_pow_vote in *)
-(*         solve_lift ret_both tt (* assign body todo(term) *) : both (*1*)(L2:|:fset [vote_result_loc]) (I2) ('unit))) (ret_both (tt : 'unit)) in *)
-(*     letb tally loc(tally_loc) := ret_both (0 : int32) in *)
-(*     letb curr loc(curr_loc) := f_field_zero (ret_both (tt : 'unit)) in *)
-(*     letb _ := foldi_both_list (f_into_iter (Build_t_Range (f_start := ret_both (0 : int32)) (f_end := cast_int (WS2 := U32) n))) (fun i => *)
-(*       ssp (fun _ => *)
-(*         letb _ := ifb (f_g_pow curr) =.? vote_result *)
-(*         then letb _ := letb tally loc(tally_loc) := i in *)
-(*         solve_lift ret_both tt (* assign body todo(term) *) in *)
-(*         ret_both (tt : 'unit) *)
-(*         else solve_lift (ret_both tt) in *)
-(*         letb _ := letb curr loc(curr_loc) := f_add curr (f_field_one (ret_both (tt : 'unit))) in *)
-(*         solve_lift ret_both tt (* assign body todo(term) *) in *)
-(*         solve_lift (ret_both (tt : 'unit)) : both (*2*)(fset [curr_loc;vote_result_loc]) ((fset [])) ('unit))) (ret_both (tt : 'unit)) in *)
-(*     letb tally_votes_state_ret loc(tally_votes_state_ret_loc) := f_clone state in *)
-(*     letb _ := letb tally_votes_state_ret loc(tally_votes_state_ret_loc) := Build_t_OvnContractState[tally_votes_state_ret] (f_tally := tally) in *)
-(*     solve_lift ret_both  tt (* assign body todo(term) *) in *)
-(*     Result_Ok (solve_lift (prod_b (f_accept (* (ret_both (tt : 'unit)) *),tally_votes_state_ret))) : both (L1 :|: L2 :|: fset [curr_loc;tally_loc;tally_votes_state_ret_loc;vote_result_loc;prod1_loc;prod2_loc] (* :|: f_clone_loc :|: f_eq_loc :|: f_into_iter_loc :|: f_end_loc :|: f_start_loc :|: f_accept_loc *) :|: f_g_pow_loc :|: f_group_one_loc :|: f_prod_loc :|: f_add_loc :|: f_field_one_loc :|: f_field_zero_loc) (I1 :|: I2) (t_Result ((v_A × t_OvnContractState (v_Z := v_Z) (v_G := v_G) (n := n)(* (both (fset []) (fset []) (uint_size)) *))) (t_ParseError)). *)
+(*         solve_lift (ifb (* not *) negb (schnorr_zkp_validate ((f_g_pow_xis state).a[i]) ((f_zkp_xis state).a[i])) *)
+(*         then letm[choice_typeMonad.result_bind_code (t_Result ((v_A × t_OvnContractState (v_Z := v_Z) (v_G := v_G) (n := n)(* (both (fset []) (fset []) (uint_size)) *))) (t_ParseError))] hoist4 := v_Break (Result_Err _ (* ParseError *)) in *)
+(*         ControlFlow_Continue (never_to_any hoist4) *)
+(*         else Result_Ok (solve_lift ret_both tt)) : both (*0*)(L2:|:fset []) (I2) (* ((* t_ControlFlow *) t_Result (t_Result ((v_A × t_OvnContractState (v_Z := v_Z) (v_G := v_G) (n := n)(* (both (fset []) (fset []) (uint_size)) *))) (t_ParseError)) ('unit)) *) _)) (Result_Ok (solve_lift ret_both (tt : 'unit))) in *)
+(*     letb g_pow_yi := compute_g_pow_yi (cast_int (WS2 := U32) (f_cvp_i params)) (f_g_pow_xis state) in *)
+(*     letb g_pow_xi_yi_vi := compute_group_element_for_vote (f_cvp_xi params) (f_cvp_vote params) g_pow_yi in *)
+(*     letb commit_vi := commit_to g_pow_xi_yi_vi in *)
+(*     letb commit_to_vote_state_ret loc(commit_to_vote_state_ret_loc) := f_clone state in *)
+(*     letb _ := letb commit_to_vote_state_ret loc(commit_to_vote_state_ret_loc) := Build_t_OvnContractState[commit_to_vote_state_ret] (f_commit_vis := update_at_usize (f_commit_vis commit_to_vote_state_ret) (cast_int (WS2 := U32) (f_cvp_i params)) commit_vi) in *)
+(*     solve_lift ret_both tt (* assign body todo(term) *) in *)
+(*     Result_Ok (prod_b (f_accept (* (ret_both (tt : 'unit)) *),commit_to_vote_state_ret))))) : both (L1 :|: L2 :|: fset [commit_to_vote_state_ret_loc;prod1_loc;prod2_loc] (* :|: f_get_loc :|: f_clone_loc :|: f_into_iter_loc :|: f_end_loc :|: f_start_loc :|: f_accept_loc :|: f_parameter_cursor_loc *)) (I1 :|: I2) (t_Result ((v_A × t_OvnContractState (v_Z := v_Z) (v_G := v_G) (n := n)(* (both (fset []) (fset []) (uint_size)) *))) (t_ParseError)). *)
+(* Admit Obligations. *)
 (* Fail Next Obligation. *)
-(* TODO *)
+
+(* Equations init_ovn_contract {L1 : {fset Location}} {I1 : Interface} {v_Z : _} {v_G : _} {n : both (fset []) (fset []) (uint_size)} `{ t_Sized (v_Z)} `{ t_Sized (v_G)} `{ t_Z_Field (v_Z)} `{ t_Group (v_G) (v_Z)} (_ : both L1 I1 ('unit)) : both (L1 (* :|: f_or_zkp_a1_loc :|: f_or_zkp_a2_loc :|: f_or_zkp_b1_loc :|: f_or_zkp_b2_loc :|: f_or_zkp_c_loc :|: f_or_zkp_d1_loc :|: f_or_zkp_d2_loc :|: f_or_zkp_r1_loc :|: f_or_zkp_r2_loc :|: f_or_zkp_x_loc :|: f_or_zkp_y_loc :|: f_commit_vis_loc :|: f_g_pow_xi_yi_vis_loc :|: f_g_pow_xis_loc :|: f_tally_loc :|: f_zkp_vis_loc :|: f_zkp_xis_loc :|: f_schnorr_zkp_c_loc :|: f_schnorr_zkp_u_loc :|: f_schnorr_zkp_z_loc *) :|: f_group_one_loc :|: f_field_zero_loc) I1 (t_Result (t_OvnContractState (v_Z := v_Z) (v_G := v_G) (n := n)(* (both (fset []) (fset []) (uint_size)) *)) (t_Reject)) := *)
+(*   init_ovn_contract _  := *)
+(*     Result_Ok (solve_lift (Build_t_OvnContractState (f_g_pow_xis := repeat (f_group_one (ret_both (tt : 'unit))) n) (f_zkp_xis := repeat (Build_t_SchnorrZKPCommit (f_schnorr_zkp_u := f_group_one (ret_both (tt : 'unit))) (f_schnorr_zkp_z := f_field_zero (ret_both (tt : 'unit))) (f_schnorr_zkp_c := f_field_zero (ret_both (tt : 'unit)))) n) (f_commit_vis := repeat (f_field_zero (ret_both (tt : 'unit))) n) (f_g_pow_xi_yi_vis := repeat (f_group_one (ret_both (tt : 'unit))) n) (f_zkp_vis := repeat (Build_t_OrZKPCommit (f_or_zkp_x := f_group_one (ret_both (tt : 'unit))) (f_or_zkp_y := f_group_one (ret_both (tt : 'unit))) (f_or_zkp_a1 := f_group_one (ret_both (tt : 'unit))) (f_or_zkp_b1 := f_group_one (ret_both (tt : 'unit))) (f_or_zkp_a2 := f_group_one (ret_both (tt : 'unit))) (f_or_zkp_b2 := f_group_one (ret_both (tt : 'unit))) (f_or_zkp_c := f_field_zero (ret_both (tt : 'unit))) (f_or_zkp_d1 := f_field_zero (ret_both (tt : 'unit))) (f_or_zkp_d2 := f_field_zero (ret_both (tt : 'unit))) (f_or_zkp_r1 := f_field_zero (ret_both (tt : 'unit))) (f_or_zkp_r2 := f_field_zero (ret_both (tt : 'unit)))) n) (f_tally := ret_both (0 : int32)))) : both (L1 (* :|: f_or_zkp_a1_loc :|: f_or_zkp_a2_loc :|: f_or_zkp_b1_loc :|: f_or_zkp_b2_loc :|: f_or_zkp_c_loc :|: f_or_zkp_d1_loc :|: f_or_zkp_d2_loc :|: f_or_zkp_r1_loc :|: f_or_zkp_r2_loc :|: f_or_zkp_x_loc :|: f_or_zkp_y_loc :|: f_commit_vis_loc :|: f_g_pow_xi_yi_vis_loc :|: f_g_pow_xis_loc :|: f_tally_loc :|: f_zkp_vis_loc :|: f_zkp_xis_loc :|: f_schnorr_zkp_c_loc :|: f_schnorr_zkp_u_loc :|: f_schnorr_zkp_z_loc *) :|: f_group_one_loc :|: f_field_zero_loc) I1 (t_Result (t_OvnContractState (v_Z := v_Z) (v_G := v_G) (n := n)(* (both (fset []) (fset []) (uint_size)) *)) (t_Reject)). *)
+(* Fail Next Obligation. *)
+
+(* Definition register_vote_state_ret_loc {v_Z : _} {v_G : _} {n : both (fset []) (fset []) (uint_size)} {v_A : _} {impl_574521470_ : _} `{ t_Sized (v_Z)} `{ t_Sized (v_G)} `{ t_Sized (v_A)} `{ t_Sized (impl_574521470_)} `{ t_Z_Field (v_Z)} `{ t_Group (v_G) (v_Z)} `{ t_HasActions (v_A)} `{ t_HasReceiveContext (impl_574521470_) ('unit)} : Location := *)
+(*   (t_OvnContractState (v_Z := v_Z) (v_G := v_G) (n := n)(* (both (fset []) (fset []) (uint_size)) *);4%nat). *)
+(* Equations register_vote {L1 : {fset Location}} {L2 : {fset Location}} {I1 : Interface} {I2 : Interface} {v_Z : _} {v_G : _} {n : both (fset []) (fset []) (uint_size)} {v_A : _} {impl_574521470_ : _} `{ t_Sized (v_Z)} `{ t_Sized (v_G)} `{ t_Sized (v_A)} `{ t_Sized (impl_574521470_)} `{ t_Z_Field (v_Z)} `{ t_Group (v_G) (v_Z)} `{ t_HasActions (v_A)} `{ t_HasReceiveContext (impl_574521470_) ('unit)} (ctx : both L1 I1 (impl_574521470_)) (state : both L2 I2 (t_OvnContractState (v_Z := v_Z) (v_G := v_G) (n := n)(* (both (fset []) (fset []) (uint_size)) *))) : both (L1 :|: L2 :|: fset [register_vote_state_ret_loc (n := n)] (* :|: f_get_loc :|: f_clone_loc :|: f_accept_loc :|: f_parameter_cursor_loc *) :|: f_g_pow_loc) (I1 :|: I2) (t_Result ((v_A × t_OvnContractState (v_Z := v_Z) (v_G := v_G) (n := n)(* (both (fset []) (fset []) (uint_size)) *))) (t_ParseError)) := *)
+(*   register_vote ctx state  := *)
+(*     solve_lift (run (letb '(_,out) := f_get (f_parameter_cursor ctx) in *)
+(*     letm[choice_typeMonad.result_bind_code (t_Result ((v_A × t_OvnContractState (v_Z := v_Z) (v_G := v_G) (n := n)(* (both (fset []) (fset []) (uint_size)) *))) (t_ParseError))] (params : t_RegisterParam (v_Z)) := matchb out with *)
+(*     | Result_Ok_case x => *)
+(*       letb x := ret_both ((x) (* : (t_RegisterParam (v_Z)) *)) in *)
+(*       ControlFlow_Continue (solve_lift x) *)
+(*     | Result_Err_case x => *)
+(*       letb x := ret_both ((x) : (t_ParseError)) in *)
+(*       letm[choice_typeMonad.result_bind_code (t_Result ((v_A × t_OvnContractState (v_Z := v_Z) (v_G := v_G) (n := n)(* (both (fset []) (fset []) (uint_size)) *))) (t_ParseError))] hoist5 := v_Break (Result_Err (* ParseError *) _) in *)
+(*       ControlFlow_Continue (solve_lift (never_to_any hoist5)) *)
+(*     end in *)
+(*     ControlFlow_Continue (letb g_pow_xi := f_g_pow (f_rp_xi params) in *)
+(*     letb zkp_xi := schnorr_zkp (f_rp_zkp_random params) g_pow_xi (f_rp_xi params) in *)
+(*     letb register_vote_state_ret loc(register_vote_state_ret_loc) := f_clone state in *)
+(*     letb _ := letb register_vote_state_ret loc(register_vote_state_ret_loc) := Build_t_OvnContractState[register_vote_state_ret] (f_g_pow_xis := update_at_usize (f_g_pow_xis register_vote_state_ret) (cast_int (WS2 := U32) (f_rp_i params)) g_pow_xi) in *)
+(*     solve_lift ret_both tt (* assign body todo(term) *) in *)
+(*     letb _ := letb register_vote_state_ret loc(register_vote_state_ret_loc) := Build_t_OvnContractState[register_vote_state_ret] (f_zkp_xis := update_at_usize (f_zkp_xis register_vote_state_ret) (cast_int (WS2 := U32) (f_rp_i params)) zkp_xi) in *)
+(*     solve_lift ret_both tt (* assign body todo(term) *) in *)
+(*                               Result_Ok (prod_b (f_accept (* (ret_both (tt : 'unit)) *),register_vote_state_ret))))) : both (L1 :|: L2 :|: fset [register_vote_state_ret_loc (n := n)] (* :|: f_get_loc :|: f_clone_loc :|: f_accept_loc :|: f_parameter_cursor_loc *) :|: f_g_pow_loc) (I1 :|: I2) (t_Result ((v_A × t_OvnContractState (v_Z := v_Z) (v_G := v_G) (n := n)(* (both (fset []) (fset []) (uint_size)) *))) (t_ParseError)). *)
+(* Admit Obligations. *)
+(* Fail Next Obligation. *)
+
+(* Definition curr_loc {v_Z : _} {v_G : _} {n : both (fset []) (fset []) (uint_size)} {v_A : _} {impl_574521470_ : _} `{ t_Sized (v_Z)} `{ t_Sized (v_G)} `{ t_Sized (v_A)} `{ t_Sized (impl_574521470_)} `{ t_Z_Field (v_Z)} `{ t_Group (v_G) (v_Z)} `{ t_HasActions (v_A)} `{ t_HasReceiveContext (impl_574521470_) ('unit)} : Location := *)
+(*   (f_field_type;5%nat). *)
+(* Definition tally_loc {v_Z : _} {v_G : _} {n : both (fset []) (fset []) (uint_size)} {v_A : _} {impl_574521470_ : _} `{ t_Sized (v_Z)} `{ t_Sized (v_G)} `{ t_Sized (v_A)} `{ t_Sized (impl_574521470_)} `{ t_Z_Field (v_Z)} `{ t_Group (v_G) (v_Z)} `{ t_HasActions (v_A)} `{ t_HasReceiveContext (impl_574521470_) ('unit)} : Location := *)
+(*   (int32;6%nat). *)
+(* Definition tally_votes_state_ret_loc {v_Z : _} {v_G : _} {n : both (fset []) (fset []) (uint_size)} {v_A : _} {impl_574521470_ : _} `{ t_Sized (v_Z)} `{ t_Sized (v_G)} `{ t_Sized (v_A)} `{ t_Sized (impl_574521470_)} `{ t_Z_Field (v_Z)} `{ t_Group (v_G) (v_Z)} `{ t_HasActions (v_A)} `{ t_HasReceiveContext (impl_574521470_) ('unit)} : Location := *)
+(*   (t_OvnContractState (v_Z := v_Z) (v_G := v_G) (n := n)(* (both (fset []) (fset []) (uint_size)) *);7%nat). *)
+(* Definition vote_result_loc {v_Z : _} {v_G : _} {n : both (fset []) (fset []) (uint_size)} {v_A : _} {impl_574521470_ : _} `{ t_Sized (v_Z)} `{ t_Sized (v_G)} `{ t_Sized (v_A)} `{ t_Sized (impl_574521470_)} `{ t_Z_Field (v_Z)} `{ t_Group (v_G) (v_Z)} `{ t_HasActions (v_A)} `{ t_HasReceiveContext (impl_574521470_) ('unit)} : Location := *)
+(*   (f_group_type;8%nat). *)
+(* (* Equations tally_votes {L1 : {fset Location}} {L2 : {fset Location}} {I1 : Interface} {I2 : Interface} {v_Z : _} {v_G : _} {n : both (fset []) (fset []) (uint_size)} {v_A : _} {impl_574521470_ : _} `{ t_Sized (v_Z)} `{ t_Sized (v_G)} `{ t_Sized (v_A)} `{ t_Sized (impl_574521470_)} `{ t_Z_Field (v_Z)} `{ t_Group (v_G) (v_Z)} `{ t_HasActions (v_A)} `{ t_HasReceiveContext (impl_574521470_) ('unit)} (_ : both L1 I1 (impl_574521470_)) (state : both L2 I2 (t_OvnContractState (v_Z := v_Z) (v_G := v_G) (n := n)(* (both (fset []) (fset []) (uint_size)) *))) : both (L1 :|: L2 :|: fset [curr_loc (n := n);tally_loc (n := n);tally_votes_state_ret_loc (n := n);vote_result_loc (n := n);prod1_loc (n := n);prod2_loc (n := n)] (* :|: f_clone_loc :|: f_eq_loc :|: f_into_iter_loc :|: f_end_loc :|: f_start_loc :|: f_accept_loc *) :|: f_g_pow_loc :|: f_group_one_loc :|: f_prod_loc :|: f_add_loc :|: f_field_one_loc :|: f_field_zero_loc) (I1 :|: I2) (t_Result ((v_A × t_OvnContractState (v_Z := v_Z) (v_G := v_G) (n := n)(* (both (fset []) (fset []) (uint_size)) *))) (t_ParseError)) := *) *)
+(* (*   tally_votes _ state  := *) *)
+(* (*     letb _ := foldi_both_list (f_into_iter (Build_t_Range (f_start := ret_both (0 : uint_size)) (f_end := n))) (fun i => *) *)
+(* (*       ssp (fun _ => *) *)
+(* (*         letb g_pow_yi := compute_g_pow_yi i (f_g_pow_xis state) in *) *)
+(* (*         letm[choice_typeMonad.result_bind_code (t_Result ((v_A × t_OvnContractState (v_Z := v_Z) (v_G := v_G) (n := n)(* (both (fset []) (fset []) (uint_size)) *))) (t_ParseError))] _ := ControlFlow_Continue (ifb (* not *)negb (zkp_one_out_of_two_validate g_pow_yi ((f_zkp_vis state).a[i])) *) *)
+(* (*         then letm[choice_typeMonad.result_bind_code (t_Result ((v_A × t_OvnContractState (v_Z := v_Z) (v_G := v_G) (n := n)(* (both (fset []) (fset []) (uint_size)) *))) (t_ParseError))] hoist6 := v_Break (Result_Err _ (* ParseError *)) in *) *)
+(* (*         ControlFlow_Continue (never_to_any hoist6) *) *)
+(* (*         else Result_Ok (solve_lift ret_both tt)) in *) *)
+(* (*         solve_lift (ifb (* not *)negb (check_commitment ((f_g_pow_xi_yi_vis state).a[i]) ((f_commit_vis state).a[i])) *) *)
+(* (*         then letm[choice_typeMonad.result_bind_code (t_Result ((v_A × t_OvnContractState (v_Z := v_Z) (v_G := v_G) (n := n)(* (both (fset []) (fset []) (uint_size)) *))) (t_ParseError))] hoist7 := v_Break (Result_Err (* ParseError *) _) in *) *)
+(* (*         ControlFlow_Continue (never_to_any hoist7) *) *)
+(* (*         else Result_Ok (solve_lift ret_both tt)) : both (*0*)(L2:|:fset []) (I2) _ (* (t_ControlFlow (t_Result ((v_A × t_OvnContractState (v_Z := v_Z) (v_G := v_G) (n := n)(* (both (fset []) (fset []) (uint_size)) *))) (t_ParseError)) ('unit)) *))) (Result_Ok (ret_both (tt : 'unit))) in *) *)
+(* (*     letb vote_result loc(vote_result_loc) := f_group_one (ret_both (tt : 'unit)) in *) *)
+(* (*     letb _ := foldi_both_list (f_into_iter (f_g_pow_xi_yi_vis state)) (fun g_pow_vote => *) *)
+(* (*       ssp (fun _ => *) *)
+(* (*         letb vote_result loc(vote_result_loc) := f_prod vote_result g_pow_vote in *) *)
+(* (*         solve_lift ret_both tt (* assign body todo(term) *) : both (*1*)(L2:|:fset [vote_result_loc]) (I2) ('unit))) (ret_both (tt : 'unit)) in *) *)
+(* (*     letb tally loc(tally_loc) := ret_both (0 : int32) in *) *)
+(* (*     letb curr loc(curr_loc) := f_field_zero (ret_both (tt : 'unit)) in *) *)
+(* (*     letb _ := foldi_both_list (f_into_iter (Build_t_Range (f_start := ret_both (0 : int32)) (f_end := cast_int (WS2 := U32) n))) (fun i => *) *)
+(* (*       ssp (fun _ => *) *)
+(* (*         letb _ := ifb (f_g_pow curr) =.? vote_result *) *)
+(* (*         then letb _ := letb tally loc(tally_loc) := i in *) *)
+(* (*         solve_lift ret_both tt (* assign body todo(term) *) in *) *)
+(* (*         ret_both (tt : 'unit) *) *)
+(* (*         else solve_lift (ret_both tt) in *) *)
+(* (*         letb _ := letb curr loc(curr_loc) := f_add curr (f_field_one (ret_both (tt : 'unit))) in *) *)
+(* (*         solve_lift ret_both tt (* assign body todo(term) *) in *) *)
+(* (*         solve_lift (ret_both (tt : 'unit)) : both (*2*)(fset [curr_loc;vote_result_loc]) ((fset [])) ('unit))) (ret_both (tt : 'unit)) in *) *)
+(* (*     letb tally_votes_state_ret loc(tally_votes_state_ret_loc) := f_clone state in *) *)
+(* (*     letb _ := letb tally_votes_state_ret loc(tally_votes_state_ret_loc) := Build_t_OvnContractState[tally_votes_state_ret] (f_tally := tally) in *) *)
+(* (*     solve_lift ret_both  tt (* assign body todo(term) *) in *) *)
+(* (*     Result_Ok (solve_lift (prod_b (f_accept (* (ret_both (tt : 'unit)) *),tally_votes_state_ret))) : both (L1 :|: L2 :|: fset [curr_loc;tally_loc;tally_votes_state_ret_loc;vote_result_loc;prod1_loc;prod2_loc] (* :|: f_clone_loc :|: f_eq_loc :|: f_into_iter_loc :|: f_end_loc :|: f_start_loc :|: f_accept_loc *) :|: f_g_pow_loc :|: f_group_one_loc :|: f_prod_loc :|: f_add_loc :|: f_field_one_loc :|: f_field_zero_loc) (I1 :|: I2) (t_Result ((v_A × t_OvnContractState (v_Z := v_Z) (v_G := v_G) (n := n)(* (both (fset []) (fset []) (uint_size)) *))) (t_ParseError)). *) *)
+(* (* Fail Next Obligation. *) *)
+(* (* TODO *) *)
 
 (** Concert lib part **)
 From ConCert.Utils Require Import Extras.
